# baseURI: https://w3id.org/knowledge-engine/devices/
# imports: https://saref.etsi.org/core/v3.1.1/
# imports: https://w3id.org/knowledge-engine

@prefix : <https://w3id.org/knowledge-engine/devices/> .
@prefix ke: <https://w3id.org/knowledge-engine/> .
@prefix owl: <http://www.w3.org/2002/07/owl#> .
@prefix rdf: <http://www.w3.org/1999/02/22-rdf-syntax-ns#> .
@prefix rdfs: <http://www.w3.org/2000/01/rdf-schema#> .
@prefix saref: <https://saref.etsi.org/core/> .
@prefix xsd: <http://www.w3.org/2001/XMLSchema#> .

:
  a owl:Ontology ;
  owl:imports <https://saref.etsi.org/core/v3.1.1/> ;
  owl:imports <https://w3id.org/knowledge-engine> ;
  owl:versionInfo "Created with TopBraid Composer" ;
.
:DeviceAccessChange
  a owl:Class ;
  rdfs:comment "An instance of this class signifies a change in the access policy of a device. The linked device (hasResource) is now accessible OR no longer accessible by the linked consumer (hasConsumer)." ;
  rdfs:label "Device access change" ;
  rdfs:subClassOf owl:Thing ;
.
:DeviceUseIntent
  a owl:Class ;
  rdfs:comment "An instance of this class declares an intention to use devices that support the specified function(s) linked with useFunction." ;
  rdfs:label "Device use intent" ;
  rdfs:subClassOf owl:Thing ;
.
:hasAccessTo
  a owl:ObjectProperty ;
  rdfs:comment "This property declares that the subject Knowledge Base has access to the object Knowledge Base, meaning that the object Knowledge Base should process incoming requests from the subject Knowledge Base." ;
  rdfs:domain ke:KnowledgeBase ;
  rdfs:label "has access to" ;
  rdfs:range ke:KnowledgeBase ;
.
:hasConsumer
  a owl:ObjectProperty ;
  rdfs:comment "Attaching a Knowledge Base to a Device Access Change with this property, means that the new policy will be enforced for the Knowledge Base in question. Meaning that the Knowledge Base may or may not consume a given resource afther the Device Access Change has been enforced." ;
  rdfs:domain :DeviceAccessChange ;
  rdfs:label "has consumer" ;
  rdfs:range ke:KnowledgeBase ;
.
:hasDeviceUseIntent
  a owl:ObjectProperty ;
  rdfs:comment "This property is used to express that a Knowledge Base has an intention to use devices of some kind. The intention can be further specified with :useFunction to only express intention to use devices that support specific Functions." ;
  rdfs:domain ke:KnowledgeBase ;
  rdfs:label "has device use intent" ;
  rdfs:range :DeviceUseIntent ;
.
:hasRegistrationURI
  a owl:DatatypeProperty ;
  rdfs:domain ke:KnowledgeBase ;
  rdfs:label "has registration URI" ;
  rdfs:range xsd:anyURI ;
.
:hasResource
  a owl:ObjectProperty ;
  rdfs:comment "This property states the resource that is being protected by a policy." ;
  rdfs:domain :DeviceAccessChange ;
  rdfs:label "has resource" ;
  rdfs:range ke:KnowledgeBase ;
.
:newAccessStatus
  a owl:DatatypeProperty ;
  rdfs:comment "This data property denotes whether or not the new policy should give access (true) or deny access (false)." ;
  rdfs:domain :DeviceAccessChange ;
  rdfs:label "new access status" ;
  rdfs:range xsd:boolean ;
.
:useFunction
  a owl:ObjectProperty ;
  rdfs:comment "This object property declares that an intention requires the use of the linked function." ;
  rdfs:label "use function" ;
  rdfs:range saref:Function ;
.
